Establish simplification of external (b3_part 0) three

exbScript.sml
@@ -21,6 +21,32 @@ open HolKernel boolLib bossLib Parse dep_rewrite
 
 val _ = new_theory"exb";
 
+(* these could be used elsewhere *)
+
+Definition encode_repfn_def:
+  encode_repfn b q = encode_function (IMAGE encode_set b)
+    (restrict (q o decode_set) (IMAGE encode_set b))
+End
+
+Theorem encode_repfn_in_repfns:
+  FINITE b ∧ EVERY_FINITE b ∧ extensional q b ⇒
+  (encode_repfn b q ∈ repfns b ⇔ is_repfn b q)
+Proof
+  rw[repfns_def, encode_repfn_def]
+  \\ reverse EQ_TAC >- metis_tac[]
+  \\ strip_tac
+  \\ fs[is_repfn_def]
+  \\ rpt strip_tac
+  \\ `q x = q' x` suffices_by rw[]
+  \\ first_x_assum(mp_tac o Q.AP_TERM`decode_function`)
+  \\ disch_then(mp_tac o C Q.AP_THM `encode_set x`)
+  \\ simp[]
+  \\ rw[restrict_def]
+  \\ metis_tac[]
+QED
+
+(* -- *)
+
 Definition b3_def:
   b3 = let d = {"0";"1"} in
     IMAGE (UNCURRY STRCAT o pair$## I (UNCURRY STRCAT))
@@ -133,6 +159,680 @@ Proof
   \\ qexists_tac`if a0 = "0" then "0" else "1"`
   \\ pop_assum strip_assume_tac
   \\ rw[] \\ EVAL_TAC
+QED
+
+Definition ext0_three_def:
+  ext0_three = mk_cf <| world := b3;
+    agent := IMAGE (UNCURRY STRCAT) ({"0";"1"} × b3);
+    env := IMAGE (UNCURRY STRCAT) ({"0";"1"} × {"0";"1"});
+    eval := λa e. SNOC (EL (ORD (EL 1 e) - ORD #"0" +
+                        2 * (ORD (EL 0 e) - ORD #"0")) a) e
+    |>
+End
+
+Theorem ext0_three_agent_eq = EVAL``ext0_three.agent``
+Theorem ext0_three_env_eq = EVAL``ext0_three.env``
+
+Theorem cf_matrix_ext0_three:
+  cf_matrix (ext0_three) =
+  [["000";"010";"100";"110"];
+   ["000";"010";"100";"111"];
+   ["000";"010";"101";"110"];
+   ["000";"010";"101";"111"];
+   ["000";"011";"100";"110"];
+   ["000";"011";"100";"111"];
+   ["000";"011";"101";"110"];
+   ["000";"011";"101";"111"];
+   ["001";"010";"100";"110"];
+   ["001";"010";"100";"111"];
+   ["001";"010";"101";"110"];
+   ["001";"010";"101";"111"];
+   ["001";"011";"100";"110"];
+   ["001";"011";"100";"111"];
+   ["001";"011";"101";"110"];
+   ["001";"011";"101";"111"]]
+Proof
+  rw[cf_matrix_def]
+  \\ rw[ext0_three_agent_eq, ext0_three_env_eq]
+  \\ qsort_set_to_list_tac
+  \\ EVAL_TAC
+QED
+
+Theorem ext0_three_in_chu_objects[simp]:
+  ext0_three ∈ chu_objects b3
+Proof
+  rw[ext0_three_def, in_chu_objects, finite_cf_def]
+  \\ rw[image_def, SUBSET_DEF, PULL_EXISTS, EXISTS_PROD]
+  \\ pop_assum mp_tac \\ rw[b3_eq] \\ rw[]
+QED
+
+Definition unevcn_def:
+  unevcn d0 s =
+    let s = if d0 = #"0" then TAKE 2 s else DROP 2 s in
+    if s = "00" then "0" else
+    if s = "01" then "c" else
+    if s = "10" then "n" else
+    "1"
+End
+
+Theorem evcn_in:
+  x ∈ {#"0";#"1"} ∧ c ∈ {"c";"n";"0";"1"} ⇒
+  evcn c x ∈ {#"0";#"1"}
+Proof
+  rw[evcn_def] \\ rw[]
+QED
+
+Theorem three_eval:
+  three.eval a e =
+  if a ∈ three.agent ∧ e ∈ three.env then
+      let d0 = HD (FST (decode_pair a)) in
+      let d1 = evcn e d0 in
+      let d2 = evcn  (SND (decode_pair a)) d1 in
+        [d0;d1;d2]
+  else ARB
+Proof
+  rw[three_def, mk_cf_def, restrict_def]
+QED
+
+Theorem ext0_three_eval:
+  ext0_three.eval a e =
+  if a ∈ ext0_three.agent ∧ e ∈ ext0_three.env then
+    SNOC (EL (ORD (EL 1 e) - ORD #"0" + TWICE (ORD (EL 0 e) - ORD #"0")) a) e
+  else ARB
+Proof
+  rw[ext0_three_def, mk_cf_def, restrict_def]
+QED
+
+Theorem b3_where_inj:
+  (i < 3) ∧ d ∈ {#"0";#"1"} ∧ d' ∈ {#"0";#"1"} ⇒
+  (b3_where i d = b3_where i d' ⇔ (d = d'))
+Proof
+  strip_tac
+  \\ rw[b3_where_def, Once EXTENSION]
+  \\ EQ_TAC \\ simp[]
+  \\ fs[lt3, b3_eq]
+  \\ metis_tac[
+       listTheory.EL,
+       EVAL``EL 0 [a;b;c]``,
+       EVAL``EL 1 [a;b;c]``,
+       EVAL``EL 2 [a;b;c]``,
+       EVAL``#"0"=#"1"``]
+QED
+
+Theorem three_eval_b3_part_0:
+  p ∈ three.agent ∧ e ∈ three.env ⇒
+  (@w. w ∈ b3_part 0 ∧ three.eval p e ∈ w) =
+  b3_where 0 (HD(FST (decode_pair p)))
+Proof
+  strip_tac
+  \\ SELECT_ELIM_TAC
+  \\ conj_tac >- metis_tac[b3_part_partitions, EVAL``0 < 3``, partitions_thm,
+                           three_in_chu_objects, in_chu_objects, wf_def]
+  \\ simp[three_eval]
+  \\ rw[b3_part_def]
+  \\ DEP_REWRITE_TAC[b3_where_inj]
+  \\ simp[]
+  \\ fs[b3_where_def]
+QED
+
+Theorem EL_4:
+  f0 ∈ {#"0";#"1"} ∧
+  f1 ∈ {#"0";#"1"}
+  ⇒
+  EL (ORD f1 - 48 + TWICE (ORD f0 - 48))
+    ((f #"0" #"0")::(f #"0" #"1")::(f #"1" #"0")::(f #"1" #"1")::"")
+  = f f0 f1
+Proof
+  rw[] \\ rw[]
+QED
+
+Theorem evcn_idem:
+  c ∈ three.env ∧ x ∈ {#"0";#"1"} ⇒
+  evcn (evcn c x :: []) x =
+  evcn c x
+Proof
+  rw[evcn_def] \\ gs[]
+  \\ gs[three_def]
+QED
+
+Theorem homotopy_equiv_ext0_three:
+  external (b3_part 0) three ≃ ext0_three -: b3
+Proof
+  rw[homotopy_equiv_def]
+  \\ qexists_tac`mk_chu_morphism (external (b3_part 0) three) ext0_three
+      <| map_agent :=
+          λq.
+          (*
+          q - pick representative (1st, (2nd -> 3rd)) given an equivalence
+              class of all such agents that fix the 1st digit
+          want: choice of 3rd for all (1st, 2nd)
+          strategy, for each (1st, 2nd),
+            let (1st', func) = q (equiv_class_for (1st, K 0))
+            in func 2nd
+          *)
+          MAP (λe.
+            let fp = fn_part three.agent three.env three.eval (b3_part 0) in
+            let p = encode_pair ([EL 0 e], "0") in
+            let a = decode_function q (encode_set (fp p)) in
+            evcn (SND (decode_pair a)) (EL 1 e))
+            ["00";"01";"10";"11"];
+         map_env := λe.
+           encode_pair (encode_set
+             (fn_part three.agent three.env three.eval (b3_part 0)
+               (encode_pair ([EL 0 e], "0"))),
+              [EL 1 e]) |>`
+  \\ qmatch_goalsub_abbrev_tac`homotopic _ (_ o h -: _) _`
+  \\ qexists_tac`mk_chu_morphism ext0_three (external (b3_part 0) three) <|
+       map_agent := λa.
+         let fp = fn_partition three.agent three.env three.eval (b3_part 0) in
+         encode_repfn fp
+         (restrict (λs.
+             let d0 = FST (decode_pair (CHOICE s)) in
+             encode_pair (d0, unevcn (HD d0) a)) fp);
+       map_env := λp.
+         let d0 = HD(FST(decode_pair(CHOICE(decode_set(FST(decode_pair p)))))) in
+         let d1 = evcn (SND(decode_pair p)) d0 in
+         [d0; d1] |>`
+  \\ qmatch_goalsub_abbrev_tac`homotopic _ (g o h -: _) _`
+  \\ `partitions (b3_part 0) b3` by simp[b3_part_partitions]
+  \\ qmatch_asmsub_abbrev_tac`LET _ fp`
+  \\ `partitions fp three.agent`
+  by(
+    qunabbrev_tac`fp`
+    \\ irule partitions_fn_partition
+    \\ qexists_tac`b3`
+    \\ simp[]
+    \\ metis_tac[three_in_chu_objects, in_chu_objects, wf_def])
+  \\ drule partitions_FINITE
+  \\ impl_keep_tac >- simp[three_def]
+  \\ strip_tac
+  \\ conj_asm1_tac
+  >- (
+    simp[maps_to_in_chu, Abbr`h`, b3_part_partitions]
+    \\ simp[is_chu_morphism_def, mk_chu_morphism_def]
+    \\ simp[restrict_def]
+    \\ conj_asm1_tac
+    >- (
+      simp[external_def, cf_external_def]
+      \\ gen_tac \\ strip_tac
+      \\ conj_tac
+      >- (
+        qmatch_goalsub_abbrev_tac`encode_set s`
+        \\ qexists_tac`s` \\ simp[]
+        \\ simp[Abbr`s`, Abbr`fp`, fn_partition_def]
+        \\ qmatch_goalsub_abbrev_tac`_ x = _ ∧ _`
+        \\ qexists_tac`x` \\ simp[]
+        \\ simp[Abbr`x`]
+        \\ simp[three_def]
+        \\ pop_assum mp_tac
+        \\ rw[ext0_three_env_eq] \\ simp[])
+      \\ pop_assum mp_tac
+      \\ rw[ext0_three_env_eq] \\ simp[three_def])
+    \\ conj_asm1_tac
+    >- (
+      simp[external_def, cf_external_def]
+      \\ simp[repfns_def]
+      \\ gen_tac \\ strip_tac
+      \\ qmatch_goalsub_abbrev_tac`encode_set (f _)`
+      \\ simp[ext0_three_def, EXISTS_PROD, b3_def]
+      \\ qmatch_goalsub_abbrev_tac`a0::b::c::d`
+      \\ qexists_tac`[a0]` \\ simp[PULL_EXISTS]
+      \\ qexists_tac`[b]` \\ simp[]
+      \\ qexists_tac`[c]` \\ simp[]
+      \\ simp[Abbr`d`]
+      \\ qmatch_goalsub_abbrev_tac`evcn d _`
+      \\ simp[Abbr`c`]
+      \\ simp[Abbr`b`]
+      \\ qmatch_goalsub_abbrev_tac`evcn b _`
+      \\ simp[Abbr`a0`]
+      \\ ntac 2 (pop_assum mp_tac)
+      \\ simp[restrict_def]
+      \\ qmatch_goalsub_abbrev_tac`encode_set s`
+      \\ `s ∈ fp`
+      by (
+        simp[Abbr`s`, Abbr`fp`, fn_partition_def]
+        \\ simp[three_def, PULL_EXISTS, EXISTS_PROD]
+        \\ metis_tac[])
+      \\ reverse IF_CASES_TAC >- metis_tac[] \\ pop_assum kall_tac
+      \\ simp[Abbr`s`]
+      \\ qmatch_goalsub_abbrev_tac`encode_set s`
+      \\ `s ∈ fp`
+      by (
+        simp[Abbr`s`, Abbr`fp`, fn_partition_def]
+        \\ simp[three_def, PULL_EXISTS, EXISTS_PROD]
+        \\ metis_tac[])
+      \\ reverse IF_CASES_TAC >- metis_tac[] \\ pop_assum kall_tac
+      \\ simp[Abbr`s`]
+      \\ qmatch_goalsub_abbrev_tac`q f1`
+      \\ `q f1 ∈ f1` by metis_tac[is_repfn_def]
+      \\ strip_tac
+      \\ qmatch_goalsub_abbrev_tac`q f2`
+      \\ `q f2 ∈ f2` by metis_tac[is_repfn_def]
+      \\ strip_tac
+      \\ `f1 ⊆ three.agent` by simp[SUBSET_DEF, Abbr`f1`, Abbr`f`, fn_part_def]
+      \\ `f2 ⊆ three.agent` by simp[SUBSET_DEF, Abbr`f2`, Abbr`f`, fn_part_def]
+      \\ `q f1 ∈ three.agent ∧ q f2 ∈ three.agent` by metis_tac[SUBSET_DEF]
+      \\ `b ∈ three.env ∧ d ∈ three.env`
+      by (
+        ntac 2 (pop_assum mp_tac)
+        \\ simp[three_def, EXISTS_PROD, Abbr`b`, Abbr`d`]
+        \\ rpt strip_tac \\ simp[] )
+      \\ rpt conj_tac \\ irule(SIMP_RULE(srw_ss())[]evcn_in)
+      \\ ntac 2 (pop_assum mp_tac)
+      \\ simp[three_def]
+      \\ PROVE_TAC[])
+    \\ simp[ext0_three_eval]
+    \\ simp[external_eval]
+    \\ rpt gen_tac
+    \\ qmatch_goalsub_abbrev_tac`encode_set (ft _)`
+    \\ strip_tac
+    \\ `∃f0 f1. f = f0::f1::[] ∧ f0 ∈ {#"0";#"1"} ∧ f1 ∈ {#"0";#"1"}`
+    by (
+      qpat_x_assum`f ∈ _`mp_tac
+      \\ simp[ext0_three_env_eq]
+      \\ strip_tac \\ simp[] )
+    \\ simp[]
+    \\ qmatch_goalsub_abbrev_tac`ft p`
+    \\ `p ∈ three.agent`
+    by ( simp[Abbr`p`, three_def] \\ fs[] )
+    \\ `ft p ∈ fp`
+    by ( simp[Abbr`fp`, fn_partition_def] \\ metis_tac[] )
+    \\ qpat_x_assum`a ∈ _`mp_tac
+    \\ simp[external_def, cf_external_def]
+    \\ simp[repfns_def] \\ strip_tac
+    \\ simp[]
+    \\ simp[Once restrict_def]
+    \\ reverse IF_CASES_TAC >- metis_tac[] \\ pop_assum kall_tac
+    \\ qunabbrev_tac`p`
+    \\ qmatch_goalsub_abbrev_tac`encode_set (ft p)`
+    \\ `p ∈ three.agent`
+    by ( simp[Abbr`p`, three_def] \\ fs[] )
+    \\ `ft p ∈ fp`
+    by ( simp[Abbr`fp`, fn_partition_def] \\ metis_tac[] )
+    \\ simp[Once restrict_def]
+    \\ reverse IF_CASES_TAC >- metis_tac[] \\ pop_assum kall_tac
+    \\ qunabbrev_tac`p`
+    \\ simp[Once restrict_def]
+    \\ reverse IF_CASES_TAC >- metis_tac[] \\ pop_assum kall_tac
+    \\ qmatch_goalsub_abbrev_tac`encode_set (ft p)`
+    \\ `p ∈ three.agent`
+    by ( simp[Abbr`p`, three_def] \\ fs[] )
+    \\ `ft p ∈ fp`
+    by ( simp[Abbr`fp`, fn_partition_def] \\ metis_tac[] )
+    \\ simp[Once restrict_def]
+    \\ reverse IF_CASES_TAC >- metis_tac[] \\ pop_assum kall_tac
+    \\ qunabbrev_tac`p`
+    \\ simp[Once restrict_def]
+    \\ reverse IF_CASES_TAC >- metis_tac[] \\ pop_assum kall_tac
+    \\ qmatch_goalsub_abbrev_tac`f0::f1::f2::[]`
+    \\ simp[three_eval]
+    \\ qmatch_goalsub_abbrev_tac`q ft0 ∈ _`
+    \\ `q ft0 ∈ ft0` by metis_tac[is_repfn_def]
+    \\ `ft0 ⊆ three.agent` by simp[Abbr`ft0`, Abbr`ft`, SUBSET_DEF, fn_part_def]
+    \\ reverse IF_CASES_TAC
+    >- (
+      `F` suffices_by rw[]
+      \\ pop_assum mp_tac
+      \\ simp[]
+      \\ conj_tac >- metis_tac[SUBSET_DEF]
+      \\ qpat_x_assum`f1 ∈ _`mp_tac
+      \\ simp[three_def]
+      \\ PROVE_TAC[])
+    \\ `FST (decode_pair (q ft0)) = [f0]`
+    by (
+      qmatch_goalsub_abbrev_tac`decode_pair p`
+      \\ qpat_x_assum`p ∈ _`mp_tac
+      \\ simp[Abbr`ft0`, Abbr`ft`]
+      \\ simp[fn_part_def]
+      \\ simp[three_eval_b3_part_0]
+      \\ DEP_REWRITE_TAC[b3_where_inj]
+      \\ qpat_x_assum`p ∈ _ ∧ _`strip_assume_tac
+      \\ qpat_x_assum`p ∈ _`mp_tac
+      \\ simp[three_def, PULL_EXISTS, EXISTS_PROD]
+      \\ rpt gen_tac
+      \\ simp[CONJ_ASSOC]
+      \\ disch_then (mp_tac o CONJUNCT1)
+      \\ rw[] \\ rw[])
+    \\ simp[]
+    \\ conj_asm1_tac
+    >- (
+      simp[evcn_def]
+      \\ qpat_x_assum`f1 ∈ _`mp_tac
+      \\ simp[]
+      \\ strip_tac \\ simp[] )
+    \\ simp[]
+    \\ qpat_x_assum`Abbrev(f2 = _)`mp_tac
+    \\ qho_match_abbrev_tac`(Abbrev(f2 = EL _ ((fx ("0","0") #"0") :: _))) ⇒ _`
+    \\ simp[]
+    \\ qabbrev_tac`fxx = λd0 d2. fx ([d0], "0") d2`
+    \\ simp[]
+    \\ simp[EL_4]
+    \\ strip_tac
+    \\ simp[Abbr`f2`]
+    \\ simp[Abbr`fxx`, Abbr`fx`])
+  \\ conj_asm1_tac
+  >- (
+    simp[maps_to_in_chu, Abbr`g`, b3_part_partitions]
+    \\ simp[is_chu_morphism_def, mk_chu_morphism_def]
+    \\ simp[restrict_def]
+    \\ conj_asm1_tac
+    >- (
+      simp[ext0_three_def, PULL_EXISTS, EXISTS_PROD]
+      \\ simp[external_def, cf_external_def, PULL_EXISTS, EXISTS_PROD]
+      \\ qx_genl_tac[`d1`,`d0`] \\ strip_tac
+      \\ qexists_tac`FST (decode_pair (CHOICE d0))`
+      \\ simp[]
+      \\ qpat_x_assum`d0 ∈ _`mp_tac
+      \\ simp[Abbr`fp`, fn_partition_def]
+      \\ strip_tac
+      \\ `CHOICE d0 ∈ d0`
+      by (
+        irule CHOICE_DEF
+        \\ simp[GSYM MEMBER_NOT_EMPTY]
+        \\ simp[fn_part_def]
+        \\ qexists_tac`x` \\ simp[] )
+      \\ `d0 ⊆ three.agent`
+      by simp[fn_part_def, SUBSET_DEF]
+      \\ `CHOICE d0 ∈ three.agent` by metis_tac[SUBSET_DEF]
+      \\ pop_assum mp_tac
+      \\ simp_tac(srw_ss())[three_def, PULL_EXISTS, EXISTS_PROD]
+      \\ qpat_x_assum`d1 ∈ _`mp_tac
+      \\ simp_tac(srw_ss())[three_def]
+      \\ simp[evcn_def]
+      \\ rw[] )
+    \\ conj_asm1_tac
+    >- (
+      simp[external_def, cf_external_def]
+      \\ rpt strip_tac
+      \\ DEP_REWRITE_TAC[encode_repfn_in_repfns]
+      \\ simp[]
+      \\ conj_asm1_tac
+      >- simp[extensional_def]
+      \\ simp[is_repfn_def]
+      \\ gen_tac \\ strip_tac
+      \\ `CHOICE s ∈ s`
+      by (
+        irule CHOICE_DEF
+        \\ simp[GSYM MEMBER_NOT_EMPTY]
+        \\ pop_assum mp_tac
+        \\ simp[Abbr`fp`, fn_partition_def, PULL_EXISTS]
+        \\ rpt strip_tac
+        \\ simp[fn_part_def]
+        \\ qexists_tac`x` \\ simp[] )
+      \\ `s ⊆ three.agent`
+      by (
+        fs[Abbr`fp`, fn_partition_def]
+        \\ simp[fn_part_def, SUBSET_DEF] )
+      \\ `CHOICE s ∈ three.agent` by metis_tac[SUBSET_DEF]
+      \\ qmatch_goalsub_abbrev_tac`decode_pair p`
+      \\ qpat_x_assum`s ∈ fp`mp_tac
+      \\ simp[Abbr`fp`, fn_partition_def]
+      \\ strip_tac
+      \\ qmatch_goalsub_abbrev_tac`pa ∈ s`
+      \\ `pa ∈ three.agent`
+      by (
+        simp[Abbr`pa`, three_def]
+        \\ qpat_x_assum`p ∈ _`mp_tac
+        \\ simp[three_def, PULL_EXISTS, EXISTS_PROD]
+        \\ rpt gen_tac \\ disch_then assume_tac
+        \\ simp[unevcn_def]
+        \\ metis_tac[])
+      \\ qpat_x_assum`p ∈ s`mp_tac
+      \\ simp[fn_part_def]
+      \\ simp[three_eval_b3_part_0]
+      \\ rpt strip_tac
+      \\ DEP_REWRITE_TAC[b3_where_inj]
+      \\ simp[Abbr`pa`]
+      \\ qpat_x_assum`p ∈ _`mp_tac
+      \\ simp[three_def, PULL_EXISTS, EXISTS_PROD]
+      \\ rw[] \\ rw[])
+    \\ simp[ext0_three_eval]
+    \\ simp[external_eval]
+    \\ simp[external_def, cf_external_def, PULL_EXISTS, EXISTS_PROD]
+    \\ qx_genl_tac[`a`,`e`,`s`] \\ strip_tac
+    \\ qmatch_goalsub_abbrev_tac`encode_repfn fp q`
+    \\ first_x_assum(qspec_then`a`mp_tac)
+    \\ simp[external_def, cf_external_def]
+    \\ DEP_REWRITE_TAC[encode_repfn_in_repfns]
+    \\ simp[]
+    \\ conj_asm1_tac >- simp[extensional_def, Abbr`q`]
+    \\ strip_tac
+    \\ simp[encode_repfn_def]
+    \\ simp[restrict_def]
+    \\ reverse IF_CASES_TAC >- metis_tac[]
+    \\ pop_assum kall_tac
+    \\ simp[three_eval]
+    \\ `q s ∈ s` by metis_tac[is_repfn_def]
+    \\ `s ⊆ three.agent`
+    by (
+      qpat_x_assum`s ∈ _`mp_tac
+      \\ simp[Abbr`fp`, fn_partition_def, PULL_EXISTS, fn_part_def, SUBSET_DEF])
+    \\ reverse IF_CASES_TAC >- metis_tac[SUBSET_DEF]
+    \\ `CHOICE s ∈ s`
+    by (
+      irule CHOICE_DEF
+      \\ simp[GSYM MEMBER_NOT_EMPTY]
+      \\ qpat_x_assum`s ∈ _`mp_tac
+      \\ simp[Abbr`fp`, fn_partition_def, PULL_EXISTS]
+      \\ rpt strip_tac
+      \\ simp[fn_part_def]
+      \\ qexists_tac`x` \\ simp[] )
+    \\ simp[Abbr`q`]
+    \\ qmatch_goalsub_abbrev_tac`decode_pair p`
+    \\ `p ∈ three.agent` by metis_tac[SUBSET_DEF]
+    \\ pop_assum mp_tac
+    \\ qpat_x_assum`a ∈ _`mp_tac
+    \\ qpat_x_assum`e ∈ _`mp_tac
+    \\ simp[ext0_three_agent_eq, three_def, PULL_EXISTS, EXISTS_PROD]
+    \\ rpt strip_tac \\ rpt BasicProvers.VAR_EQ_TAC
+    \\ simp[evcn_def, unevcn_def])
+  \\ qpat_assum`h :- _ → _ -: _`(mp_then Any mp_tac compose_in_chu)
+  \\ disch_then(qpat_assum`g :- _ → _ -: _` o mp_then Any strip_assume_tac)
+  \\ qpat_assum`g :- _ → _ -: _`(mp_then Any mp_tac compose_in_chu)
+  \\ disch_then(qpat_assum`h :- _ → _ -: _` o mp_then Any strip_assume_tac)
+  \\ simp[homotopic_id_map_env_id]
+  \\ simp[restrict_def]
+  \\ conj_tac
+  >- (
+    simp[external_eval]
+    \\ rpt gen_tac \\ strip_tac
+    \\ irule EQ_SYM
+    \\ IF_CASES_TAC \\ simp[]
+    \\ reverse IF_CASES_TAC >- metis_tac[maps_to_in_chu, is_chu_morphism_def]
+    \\ simp[Abbr`h`, mk_chu_morphism_def]
+    \\ simp[restrict_def]
+    \\ reverse IF_CASES_TAC >- metis_tac[maps_to_in_chu, is_chu_morphism_def]
+    \\ ntac 2 (pop_assum kall_tac)
+    \\ simp[Abbr`g`, mk_chu_morphism_def]
+    \\ simp[restrict_def]
+    \\ qmatch_goalsub_abbrev_tac`three.eval f1 _ = _ f2 _`
+    \\ `f1 = f2`
+    by (
+      simp[Abbr`f1`, Abbr`f2`]
+      \\ qpat_x_assum`e ∈ _`mp_tac
+      \\ simp[external_def, cf_external_def, PULL_EXISTS, EXISTS_PROD]
+      \\ rpt gen_tac \\ strip_tac
+      \\ `CHOICE x ∈ x`
+      by (
+        irule CHOICE_DEF
+        \\ simp[GSYM MEMBER_NOT_EMPTY]
+        \\ qpat_x_assum`_ ∈ fp`mp_tac
+        \\ simp[Abbr`fp`, fn_partition_def, PULL_EXISTS]
+        \\ rpt strip_tac
+        \\ simp[fn_part_def]
+        \\ goal_assum(first_assum o mp_then Any mp_tac)
+        \\ simp[])
+      \\ `x ⊆ three.agent`
+      by (
+        fs[Abbr`fp`, fn_partition_def]
+        \\ simp[fn_part_def, SUBSET_DEF] )
+      \\ `CHOICE x ∈ three.agent` by metis_tac[SUBSET_DEF]
+      \\ qmatch_goalsub_abbrev_tac`decode_pair p`
+      \\ qpat_x_assum`x ∈ fp`mp_tac
+      \\ simp[Abbr`fp`, fn_partition_def]
+      \\ disch_then(qx_choose_then`b`strip_assume_tac)
+      \\ qpat_x_assum`p ∈ x`mp_tac
+      \\ simp[Once fn_part_def]
+      \\ simp[three_eval_b3_part_0]
+      \\ DEP_REWRITE_TAC[b3_where_inj]
+      \\ conj_tac
+      >- (
+        simp[]
+        \\ qpat_x_assum`b ∈ _`mp_tac
+        \\ qpat_x_assum`p ∈ _`mp_tac
+        \\ simp[three_def, PULL_EXISTS, EXISTS_PROD]
+        \\ rpt strip_tac \\ rw[])
+      \\ strip_tac
+      \\ AP_TERM_TAC
+      \\ AP_TERM_TAC
+      \\ simp[fn_part_def, Once EXTENSION]
+      \\ qx_gen_tac`z`
+      \\ Cases_on`z ∈ three.agent` \\ simp[]
+      \\ irule EQ_SYM
+      \\ qmatch_goalsub_abbrev_tac`three.eval pp`
+      \\ `pp ∈ three.agent`
+      by (
+        qpat_x_assum`p ∈ _`mp_tac
+        \\ simp[Abbr`pp`, three_def, PULL_EXISTS, EXISTS_PROD]
+        \\ rpt strip_tac \\ simp[] )
+      \\ simp[three_eval_b3_part_0]
+      \\ simp[Abbr`pp`]
+      \\ metis_tac[] )
+    \\ simp[Abbr`f2`]
+    \\ pop_assum (SUBST_ALL_TAC o SYM)
+    \\ simp[three_eval]
+    \\ Cases_on`f1 ∈ three.agent` \\ simp[]
+    \\ qpat_x_assum`e ∈ _`mp_tac
+    \\ simp[external_def, cf_external_def, PULL_EXISTS, EXISTS_PROD]
+    \\ rpt strip_tac
+    \\ `x ⊆ three.agent`
+    by (
+      fs[Abbr`fp`, fn_partition_def]
+      \\ simp[fn_part_def, SUBSET_DEF] )
+    \\ `CHOICE x ∈ x`
+    by (
+      irule CHOICE_DEF
+      \\ simp[GSYM MEMBER_NOT_EMPTY]
+      \\ qpat_x_assum`_ ∈ fp`mp_tac
+      \\ simp[Abbr`fp`, fn_partition_def, PULL_EXISTS]
+      \\ rpt strip_tac
+      \\ simp[fn_part_def]
+      \\ goal_assum(first_assum o mp_then Any mp_tac)
+      \\ simp[])
+    \\ reverse IF_CASES_TAC
+    >- (
+      `F` suffices_by rw[]
+      \\ pop_assum mp_tac
+      \\ `CHOICE x ∈ three.agent` by metis_tac[SUBSET_DEF]
+      \\ pop_assum mp_tac
+      \\ qpat_x_assum`_ ∈ three.env`mp_tac
+      \\ simp[evcn_def, three_def]
+      \\ rw[] \\ rw[] )
+    \\ simp[]
+    \\ reverse conj_asm1_tac >- simp[]
+    \\ fs[]
+    \\ qpat_x_assum`a ∈ _`mp_tac
+    \\ simp[external_def, cf_external_def]
+    \\ simp[repfns_def] \\ strip_tac
+    \\ simp[Abbr`f1`]
+    \\ simp[restrict_def]
+    \\ reverse IF_CASES_TAC >- metis_tac[]
+    \\ pop_assum kall_tac
+    \\ qpat_x_assum`x ∈ _`mp_tac
+    \\ simp[Abbr`fp`, fn_partition_def]
+    \\ strip_tac
+    \\ qmatch_asmsub_abbrev_tac`p ∈ x`
+    \\ qmatch_goalsub_abbrev_tac`decode_pair qp`
+    \\ qmatch_asmsub_abbrev_tac`is_repfn fp`
+    \\ `x ∈ fp` by (simp[Abbr`fp`, fn_partition_def] \\ metis_tac[])
+    \\ `qp ∈ x` by metis_tac[is_repfn_def]
+    \\ qmatch_goalsub_abbrev_tac`evcn _ y`
+    \\ qmatch_goalsub_abbrev_tac`evcn _ yy :: _`
+    \\ `yy = y`
+    by(
+      rpt(qpat_x_assum`_ ∈ x`mp_tac)
+      \\ simp[fn_part_def]
+      \\ rpt strip_tac
+      \\ ntac 2 (qhdtm_x_assum`$!`mp_tac)
+      \\ simp[three_eval_b3_part_0]
+      \\ DEP_REWRITE_TAC[b3_where_inj]
+      \\ simp[]
+      \\ ntac 3 (qpat_x_assum`_ ∈ three.agent`mp_tac)
+      \\ simp[Ntimes three_def 3, PULL_EXISTS, EXISTS_PROD]
+      \\ simp[Abbr`y`, Abbr`yy`]
+      \\ rpt gen_tac \\ strip_tac \\ rpt BasicProvers.VAR_EQ_TAC \\ simp[]
+      \\ rpt gen_tac \\ strip_tac \\ rpt BasicProvers.VAR_EQ_TAC \\ simp[]
+      \\ rpt gen_tac \\ strip_tac \\ rpt BasicProvers.VAR_EQ_TAC \\ simp[]
+      \\ srw_tac[SatisfySimps.SATISFY_ss][])
+    \\ simp[]
+    \\ irule EQ_SYM
+    \\ irule evcn_idem
+    \\ `qp ∈ three.agent` by metis_tac[SUBSET_DEF]
+    \\ pop_assum mp_tac
+    \\ simp[Abbr`y`]
+    \\ simp[three_def, PULL_EXISTS]
+    \\ rw[] \\ rw[])
+  \\ simp[ext0_three_eval]
+  \\ rpt gen_tac \\ strip_tac
+  \\ irule EQ_SYM
+  \\ IF_CASES_TAC \\ simp[]
+  \\ reverse IF_CASES_TAC >- metis_tac[maps_to_in_chu, is_chu_morphism_def]
+  \\ pop_assum kall_tac
+  \\ simp[Abbr`g`, mk_chu_morphism_def]
+  \\ simp[restrict_def]
+  \\ reverse IF_CASES_TAC >- metis_tac[maps_to_in_chu, is_chu_morphism_def]
+  \\ simp[Abbr`h`, mk_chu_morphism_def]
+  \\ simp[restrict_def]
+  \\ pop_assum kall_tac
+  \\ qmatch_goalsub_abbrev_tac`encode_set (ft e0)`
+  \\ `e0 ∈ three.agent`
+  by (
+    simp[three_def, Abbr`e0`]
+    \\ qpat_x_assum`e ∈ _`mp_tac
+    \\ simp[ext0_three_env_eq]
+    \\ strip_tac \\ simp[] )
+  \\ `ft e0 ∈ fp`
+  by (
+    simp[Abbr`fp`, fn_partition_def]
+    \\ metis_tac[] )
+  \\ simp[]
+  \\ qmatch_goalsub_abbrev_tac`d0::d1::_`
+  \\ reverse conj_asm1_tac
+  >- ( pop_assum SUBST1_TAC \\ simp[] )
+  \\ `HD e = d0`
+  by (
+    simp[Abbr`d0`]
+    \\ `CHOICE (ft e0) ∈ ft e0`
+    by (
+      irule CHOICE_DEF
+      \\ simp[GSYM MEMBER_NOT_EMPTY]
+      \\ simp[Abbr`ft`, fn_part_def]
+      \\ qexists_tac`e0`
+      \\ simp[] )
+    \\ `ft e0 ⊆ three.agent`
+    by simp[Abbr`ft`, fn_part_def, SUBSET_DEF]
+    \\ qmatch_goalsub_abbrev_tac`decode_pair p`
+    \\ `p ∈ three.agent` by metis_tac[SUBSET_DEF]
+    \\ qpat_x_assum`p ∈ ft _`mp_tac
+    \\ simp[Abbr`ft`, fn_part_def]
+    \\ simp[three_eval_b3_part_0]
+    \\ DEP_REWRITE_TAC[b3_where_inj]
+    \\ simp[]
+    \\ qpat_x_assum`_ ∈ three.agent`mp_tac
+    \\ simp[three_def, PULL_EXISTS, EXISTS_PROD]
+    \\ qpat_x_assum`_ ∈ three.agent`mp_tac
+    \\ simp[three_def, PULL_EXISTS, EXISTS_PROD]
+    \\ simp[Abbr`e0`]
+    \\ strip_tac
+    \\ rpt gen_tac \\ strip_tac \\ rpt BasicProvers.VAR_EQ_TAC \\ simp[])
+  \\ `d1 = EL 1 e`
+  by (
+    qpat_x_assum`e ∈ _`mp_tac
+    \\ simp[Abbr`d1`, ext0_three_env_eq]
+    \\ strip_tac \\ simp[evcn_def] )
+  \\ qpat_x_assum`e ∈ _`mp_tac
+  \\ simp[ext0_three_env_eq]
+  \\ strip_tac \\ fs[]
 QED
 
 val _ = export_theory();
